theories/Finite_Term_Words.thy
@@ -1,6 +1,6 @@
 theory Finite_Term_Words
   imports RRA_Digit_Use_Paths
-    Factor_Executable_Artifact_Values
+    Factor_Executable_Artifact_Values Complete_Value_References
 begin
 
 section \<open>A counted digit word delimits a sequence of prefix codes\<close>
@@ -92,61 +92,183 @@ lemma artifact_rows_word_cancel [simp]:
         pair_word_cancel[OF counted_digit_word_cancel[OF row_word_cancel(2)]
           counted_digit_word_cancel[OF row_word_cancel(2)]]]])
 
-section \<open>Every executable term has one prefix-free digit word\<close>
+section \<open>Every executable term has one prefix-free digit word over a target code\<close>
 
-fun finite_term_word :: "finite_factor_term \<Rightarrow> bool list" where
-  "finite_term_word (Finite_Payload v)=False#False#digit_address_word v"
-| "finite_term_word (Finite_Pair t u)=True#finite_term_word t@finite_term_word u"
-| "finite_term_word (Finite_Target (Finite_Whole C))=False#True#False#artifact_rows_word (finite_artifact_rows C)"
-| "finite_term_word (Finite_Target (Finite_Anchor C a))=
-    False#True#True#artifact_rows_word (finite_artifact_rows C)@digit_address_word a"
+fun finite_term_targets :: "finite_factor_term \<Rightarrow> finite_exact_target set" where
+  "finite_term_targets (Finite_Payload v)={}"
+| "finite_term_targets (Finite_Pair t u)=finite_term_targets t \<union> finite_term_targets u"
+| "finite_term_targets (Finite_Target x)={x}"
 
-lemma finite_term_word_cancel:
-  "finite_term_word t@xs=finite_term_word u@ys \<longleftrightarrow> t=u \<and> xs=ys"
-proof (induction t arbitrary: u xs ys rule: finite_term_word.induct)
+definition target_code_cancels :: "(finite_exact_target \<Rightarrow> bool list) \<Rightarrow> finite_exact_target set \<Rightarrow> bool" where
+  "target_code_cancels leaf A \<longleftrightarrow> (\<forall>x\<in>A. \<forall>y\<in>A. \<forall>u v. leaf x@u=leaf y@v \<longleftrightarrow> x=y \<and> u=v)"
+
+lemma target_code_cancels_subset:
+  "target_code_cancels leaf B \<Longrightarrow> A\<subseteq>B \<Longrightarrow> target_code_cancels leaf A"
+  by (auto simp: target_code_cancels_def)
+
+fun finite_term_word_with :: "(finite_exact_target \<Rightarrow> bool list) \<Rightarrow> finite_factor_term \<Rightarrow> bool list" where
+  "finite_term_word_with leaf (Finite_Payload v)=False#False#digit_address_word v"
+| "finite_term_word_with leaf (Finite_Pair t u)=True#finite_term_word_with leaf t@finite_term_word_with leaf u"
+| "finite_term_word_with leaf (Finite_Target x)=False#True#leaf x"
+
+lemma finite_term_word_with_cancel:
+  assumes "target_code_cancels leaf (finite_term_targets t \<union> finite_term_targets s)"
+  shows "finite_term_word_with leaf t@xs=finite_term_word_with leaf s@ys \<longleftrightarrow> t=s \<and> xs=ys"
+  using assms
+proof (induction t arbitrary: s xs ys rule: finite_term_targets.induct)
   case (1 v)
-  then show ?case by (cases u rule: finite_term_word.cases) auto
+  then show ?case by (cases s) auto
 next
   case (2 t1 t2)
   show ?case
-  proof (cases u rule: finite_term_word.cases)
-    case (2 u1 u2)
-    have "finite_term_word (Finite_Pair t1 t2)@xs=finite_term_word u@ys \<longleftrightarrow>
-        finite_term_word t1@(finite_term_word t2@xs)=finite_term_word u1@(finite_term_word u2@ys)"
-      by (simp add: 2)
-    also have "\<dots> \<longleftrightarrow> t1=u1 \<and> finite_term_word t2@xs=finite_term_word u2@ys"
-      by (rule "2.IH"(1))
-    also have "\<dots> \<longleftrightarrow> t1=u1 \<and> t2=u2 \<and> xs=ys"
-      by (simp add: "2.IH"(2))
-    finally show ?thesis by (simp add: 2)
+  proof (cases s)
+    case (Finite_Pair s1 s2)
+    have left: "target_code_cancels leaf (finite_term_targets t1 \<union> finite_term_targets s1)"
+      and right: "target_code_cancels leaf (finite_term_targets t2 \<union> finite_term_targets s2)"
+      by (rule target_code_cancels_subset[OF "2.prems"]; auto simp: Finite_Pair)+
+    have "finite_term_word_with leaf (Finite_Pair t1 t2)@xs=finite_term_word_with leaf s@ys \<longleftrightarrow>
+        finite_term_word_with leaf t1@(finite_term_word_with leaf t2@xs)=
+        finite_term_word_with leaf s1@(finite_term_word_with leaf s2@ys)"
+      by (simp add: Finite_Pair)
+    also have "\<dots> \<longleftrightarrow> t1=s1 \<and> finite_term_word_with leaf t2@xs=finite_term_word_with leaf s2@ys"
+      by (rule "2.IH"(1)[OF left])
+    also have "\<dots> \<longleftrightarrow> t1=s1 \<and> t2=s2 \<and> xs=ys"
+      by (simp add: "2.IH"(2)[OF right])
+    finally show ?thesis by (simp add: Finite_Pair)
   qed auto
 next
-  case (3 C)
-  then show ?case by (cases u rule: finite_term_word.cases) (auto simp: finite_artifact_rows_injective)
-next
-  case (4 C a)
-  then show ?case by (cases u rule: finite_term_word.cases) (auto simp: finite_artifact_rows_injective)
+  case (3 x)
+  then show ?case by (cases s) (auto simp: target_code_cancels_def)
 qed
 
-theorem finite_term_word_injective: "finite_term_word t=finite_term_word u \<longleftrightarrow> t=u"
-  using finite_term_word_cancel[of t "[]" u "[]"] by simp
+fun finite_term_word_with_fold ::
+  "(finite_exact_target \<Rightarrow> bool list) \<Rightarrow> ('s \<Rightarrow> bool \<Rightarrow> 's) \<Rightarrow> finite_factor_term \<Rightarrow> 's \<Rightarrow> 's" where
+  "finite_term_word_with_fold leaf f (Finite_Pair t u) s=
+    finite_term_word_with_fold leaf f u (finite_term_word_with_fold leaf f t (f s True))"
+| "finite_term_word_with_fold leaf f t s=foldl f s (finite_term_word_with leaf t)"
 
-fun finite_term_word_fold :: "('s \<Rightarrow> bool \<Rightarrow> 's) \<Rightarrow> finite_factor_term \<Rightarrow> 's \<Rightarrow> 's" where
-  "finite_term_word_fold f (Finite_Pair t u) s=finite_term_word_fold f u (finite_term_word_fold f t (f s True))"
-| "finite_term_word_fold f t s=foldl f s (finite_term_word t)"
+lemma finite_term_word_with_fold_exact:
+  "finite_term_word_with_fold leaf f t s=foldl f s (finite_term_word_with leaf t)"
+  by (induction leaf f t s rule: finite_term_word_with_fold.induct) simp_all
 
-theorem finite_term_word_fold_exact:
-  "finite_term_word_fold f t s=foldl f s (finite_term_word t)"
-  by (induction f t s rule: finite_term_word_fold.induct) simp_all
+section \<open>Repeated artifacts share one first-occurrence table\<close>
 
-export_code finite_term_word finite_term_word_fold checking SML
+lemma value_reference_step_set: "set (snd (value_reference_step x T))=insert x (set T)"
+proof (cases "value_reference_index x T")
+  case None
+  then show ?thesis by (simp add: value_reference_step_def)
+next
+  case (Some i)
+  have "x\<in>set T" using value_reference_index_read[OF Some] nth_mem by metis
+  then show ?thesis using Some by (auto simp: value_reference_step_def)
+qed
+
+fun finite_term_rows_onto :: "finite_factor_term \<Rightarrow> artifact_value_rows list \<Rightarrow> artifact_value_rows list" where
+  "finite_term_rows_onto (Finite_Payload v) T=T"
+| "finite_term_rows_onto (Finite_Pair t u) T=finite_term_rows_onto u (finite_term_rows_onto t T)"
+| "finite_term_rows_onto (Finite_Target x) T=
+    snd (value_reference_step (finite_artifact_rows (finite_target_artifact x)) T)"
+
+lemma finite_term_rows_onto_set:
+  "set (finite_term_rows_onto t T)=set T \<union> (finite_artifact_rows \<circ> finite_target_artifact) ` finite_term_targets t"
+  by (induction t T rule: finite_term_rows_onto.induct) (auto simp: value_reference_step_set)
+
+definition finite_term_rows :: "finite_factor_term \<Rightarrow> artifact_value_rows list" where
+  "finite_term_rows t=finite_term_rows_onto t []"
+
+definition finite_rows_index_word :: "artifact_value_rows list \<Rightarrow> finite_exact_artifact \<Rightarrow> bool list" where
+  "finite_rows_index_word T C=digit_natural_path (case value_reference_index (finite_artifact_rows C) T of
+    None \<Rightarrow> length T | Some i \<Rightarrow> i)"
+
+lemma finite_rows_index_word_cancel:
+  assumes "finite_artifact_rows C\<in>set T" "finite_artifact_rows D\<in>set T"
+  shows "finite_rows_index_word T C@u=finite_rows_index_word T D@v \<longleftrightarrow> C=D \<and> u=v"
+proof -
+  obtain i where i: "value_reference_index (finite_artifact_rows C) T=Some i"
+    using assms(1) value_reference_index_absent[of "finite_artifact_rows C" T]
+    by (cases "value_reference_index (finite_artifact_rows C) T") auto
+  obtain j where j: "value_reference_index (finite_artifact_rows D) T=Some j"
+    using assms(2) value_reference_index_absent[of "finite_artifact_rows D" T]
+    by (cases "value_reference_index (finite_artifact_rows D) T") auto
+  have same_index: "i=j \<longleftrightarrow> C=D"
+  proof
+    assume "i=j"
+    then have "finite_artifact_rows C=finite_artifact_rows D"
+      using value_reference_index_read[OF i] value_reference_index_read[OF j] by simp
+    then show "C=D" by (simp add: finite_artifact_rows_injective)
+  next
+    assume "C=D"
+    then show "i=j" using i j by simp
+  qed
+  show ?thesis by (simp add: finite_rows_index_word_def i j digit_natural_path_cancel same_index)
+qed
+
+fun finite_target_reference_word :: "artifact_value_rows list \<Rightarrow> finite_exact_target \<Rightarrow> bool list" where
+  "finite_target_reference_word T (Finite_Whole C)=False#finite_rows_index_word T C"
+| "finite_target_reference_word T (Finite_Anchor C a)=True#finite_rows_index_word T C@digit_address_word a"
+
+lemma finite_target_reference_word_cancels:
+  assumes "\<forall>x\<in>A. finite_artifact_rows (finite_target_artifact x)\<in>set T"
+  shows "target_code_cancels (finite_target_reference_word T) A"
+  unfolding target_code_cancels_def
+proof (intro ballI allI)
+  fix x y u v assume x: "x\<in>A" and y: "y\<in>A"
+  have xm: "finite_artifact_rows (finite_target_artifact x)\<in>set T" using assms x by blast
+  have ym: "finite_artifact_rows (finite_target_artifact y)\<in>set T" using assms y by blast
+  show "finite_target_reference_word T x@u=finite_target_reference_word T y@v \<longleftrightarrow> x=y \<and> u=v"
+    using xm ym by (cases x; cases y) (simp_all add: finite_rows_index_word_cancel)
+qed
+
+definition finite_term_shared_word :: "finite_factor_term \<Rightarrow> bool list" where
+  "finite_term_shared_word t=(let T=finite_term_rows t in
+    counted_digit_word artifact_rows_word T@finite_term_word_with (finite_target_reference_word T) t)"
+
+theorem finite_term_shared_word_injective:
+  "finite_term_shared_word t=finite_term_shared_word s \<longleftrightarrow> t=s"
+proof
+  assume same: "finite_term_shared_word t=finite_term_shared_word s"
+  let ?T="finite_term_rows t"
+  have parts: "finite_term_rows t=finite_term_rows s \<and>
+      finite_term_word_with (finite_target_reference_word (finite_term_rows t)) t=
+      finite_term_word_with (finite_target_reference_word (finite_term_rows s)) s"
+    using same by (simp (no_asm_use) only: finite_term_shared_word_def Let_def
+      counted_digit_word_cancel[OF artifact_rows_word_cancel])
+  have tables: "finite_term_rows s=?T" using parts by simp
+  have words: "finite_term_word_with (finite_target_reference_word ?T) t@[]=
+      finite_term_word_with (finite_target_reference_word ?T) s@[]"
+    using conjunct2[OF parts] by (simp only: tables append_Nil2)
+  have table_t: "\<forall>x\<in>finite_term_targets t. finite_artifact_rows (finite_target_artifact x)\<in>set ?T"
+    by (simp add: finite_term_rows_def finite_term_rows_onto_set)
+  have table_s: "\<forall>x\<in>finite_term_targets s. finite_artifact_rows (finite_target_artifact x)\<in>set (finite_term_rows s)"
+    by (simp add: finite_term_rows_def finite_term_rows_onto_set)
+  have members: "\<forall>x\<in>finite_term_targets t \<union> finite_term_targets s.
+      finite_artifact_rows (finite_target_artifact x)\<in>set ?T"
+    using table_t table_s tables by auto
+  show "t=s"
+    using words finite_term_word_with_cancel[OF finite_target_reference_word_cancels[OF members], of "[]" "[]"]
+    by blast
+qed simp
+
+definition finite_term_shared_word_fold :: "('s \<Rightarrow> bool \<Rightarrow> 's) \<Rightarrow> finite_factor_term \<Rightarrow> 's \<Rightarrow> 's" where
+  "finite_term_shared_word_fold f t s=(let T=finite_term_rows t in
+    finite_term_word_with_fold (finite_target_reference_word T) f t (foldl f s (counted_digit_word artifact_rows_word T)))"
+
+theorem finite_term_shared_word_fold_exact:
+  "finite_term_shared_word_fold f t s=foldl f s (finite_term_shared_word t)"
+  by (simp add: finite_term_shared_word_fold_def finite_term_shared_word_def Let_def finite_term_word_with_fold_exact)
+
+export_code finite_term_shared_word finite_term_shared_word_fold checking SML
 
 text \<open>
   Payloads and addresses use the natural digit path of their length followed by
-  the existing address digit path, so a digit word is self-delimiting. Artifact
-  rows, pairs and targets compose those words, and the prefix cancellation of
-  every component gives the cancellation of the whole term word. The fold
-  delivers the same word incrementally without materializing it.
+  the existing address digit path, so a digit word is self-delimiting. A term word
+  is parameterized by the code of its target leaves, and it cancels whenever that
+  code cancels on the targets of the compared terms. The shared word first gives
+  the rows of every distinct artifact in first-occurrence order and then codes
+  each target by the natural index of its artifact in that table; the
+  first-occurrence table of the value reference theory makes the index code
+  cancel on every artifact of the term. The fold delivers the same word
+  incrementally without materializing it.
 \<close>
 
 end
