theories/Constructed_History_Presentation.thy
@@ -1,0 +1,17 @@
+theory Constructed_History_Presentation
+  imports Quoted_History_Presentation Factor_Constructed_History_Investigation
+begin
+
+section \<open>A constructed history report keeps every producer family\<close>
+
+definition constructed_history_report_value :: "nat list \<Rightarrow> nat list list \<Rightarrow> finite_factor_term" where
+  "constructed_history_report_value ws selections=finite_pair_presentation finite_index_sequence_value
+    (finite_pair_presentation (finite_investigation_packet_value finite_candidate_context_value finite_digit_assessment_value)
+      (finite_sequence_presentation finite_digit_source_value)) (digit_history_report constructed_history_packet ws selections)"
+
+definition constructed_history_report_selections :: "nat list list" where
+  "constructed_history_report_selections=[[],[0],[0,1]]"
+
+export_code constructed_history_report_value checking SML
+
+end
