theories/Quoted_History_Presentation.thy
@@ -1,0 +1,26 @@
+theory Quoted_History_Presentation
+  imports Known_History_Presentation Factor_Quoted_History_Investigation
+begin
+
+section \<open>Additional producers keep every produced result family\<close>
+
+definition finite_candidate_context_value where
+  "finite_candidate_context_value=finite_pair_presentation finite_digit_context_value
+    (finite_sequence_presentation (finite_collection_presentation finite_digit_result_row_value))"
+
+definition quoted_history_report_value :: "nat list \<Rightarrow> nat list list \<Rightarrow> finite_factor_term" where
+  "quoted_history_report_value ws selections=finite_pair_presentation finite_index_sequence_value
+    (finite_pair_presentation (finite_investigation_packet_value finite_candidate_context_value finite_digit_assessment_value)
+      (finite_sequence_presentation finite_digit_source_value)) (digit_history_report quoted_history_packet ws selections)"
+
+definition quoted_history_report_selections :: "nat list list" where
+  "quoted_history_report_selections=[[],[0],[0,1]]"
+
+export_code quoted_history_report_value checking SML
+
+text \<open>
+  A context of the additional-producer framework keeps the digit history
+  context and the complete result family of every additional producer in order.
+\<close>
+
+end
